---
title: "Notes-on-Understanding-Analysis"
author: "Yang Ge"
date: "9/28/2017"
output:
  html_document:
    keep_md: false
    toc: true
---

# Chapter 1
## section 1.3 The Axiom of Completeness

* **_1.3.0 Axiom of Completeness_:** Every non empty set of real numbers that is bounded
  above has a least upper bound.

* **_1.3.1 Definition of LB and UB_:** $A \subseteq R$ is bounded above if there exists $b$,
such that $a \le b$ for all $a \in A$. Similar for lower bound.

* **_Lemma 1.3.8_** Assume $s \in R$ is an upper bound for a set $A \$

### Exercises

* **_Exercise 1.3.3_**

(a) For any $a \in A$, a is an upper bound of $B$, thus $\sup B <= a$. Thus $\sup B$ is a lower
bound of $A$. For any lower bound of A $b \in B, b <= \sup B$, thus $\sup B = \inf A$.
(b) The greatest lower bound can be deduced from (a)

* **_Exercise 1.3.4_**

(a) It's the $\max \sup(A_k)$.
(b) It cannot be generalized to infinite cases. Let $A_n = \{x|x \le n\}$, $\cup_{i=1}^\infty A_n = R$. It's not even bounded above.

* **_Exercise 1.3.6_**

(a) let $c \in A+B$, then $c = a+b$ for some $a \in A, b \in B$.
    Then $a \le s, b \le t$, then $a+b \le s+t$. $s+t$ is an upper bound of $A+B$.
(b) First, we show $u-a$ is a upper bound of $B$.
If $b \in B$, then $a + b \leq u$, then
    $b \leq u-a$ for $b \in B$. Then $u-a$ is an upper bound of $B$. We have $t \leq u-a$
(c) Next we show $u-t$ is an upper bound of $A$. This is because for all $a \in A$,
we have $t \leq u-a$, it means $a \leq u - t$, then $r \leq u-t$. So $r+t \leq u$.
(d) For any $\epsilon > 0$, We can find $a \in A, a > r - \epsilon / 2$ and $b \in B, b > s - \epsilon / 2$, so $a+b \in A+B$ and $a+b > r+s-\epsilon$.
    
* **_Exercise 1.3.7_**

1. $a$ is an upper bound of $A$, then $a \ge \sup A$.
2. On the other hand, $a \in A$, so $a \le \sup A$.
3. Together we have $a = \sup A$.

* **_Exercise 1.3.8_**

(a) 0, when $m = 1, n \rightarrow \inf$. 1, when $m = n-1, n \rightarrow \inf$.
(b) -1, +1
(c) 1/4, 1/3
(d) 0, 1

* **_Exercise 1.3.9_**

(a) Assume $\epsilon = \sup B - \sup A > 0$, according to lemma 1.3.8, there is $b \in B$ such
    that $b > \sup B - \epsilon = \sup A$. So $b$ is an upper bound of $A$.
(b) Let $A = [0,1], B=(0,1)$, then $\sup A = \sup B = 1$. If $b \in B$ is an upper bound of $A$,
    then $b \ge 1$, then $b \notin B$.

* **_Exercise 1.3.10 (Cut Property)_**

(a) Let $c = \sup A$. Then for $x \in A, x <= c$. For $b \in B$, because $a < b, \forall a \in A$,
    Then $b$ is an upper bound of $A$, therefore, $c \le b$.
(b) The other way. Let $B$ be the set of all upper bounds of $A$. $c$ is the cut, then $c \ge a$
    for all $a \in A$. Then $c$ is an upper bound of $A$. Let $b$ be an upper bound, then $b \in B$. Then $c \le b$, then $c = \sup A$.
(c) Let $A = \{a|a^2<2\}, B = \{b|b^2>2\}$.

* **_Exercise 1.3.11_**

(a) True. For $a \in A$, we have $a \in B$, then $a <= \sup B$. So $\sup B$ is an upper bound
    of $A$. Therefore $\sup A \le \sup B$.
(b) True. Let $c = (\sup A + \inf B) / 2$, the $\inf B > c > \sup A$. So
$$
a \le \sup A < c < \inf B \le b
$$

(c) False. Let $A = \{a| a \in \mathbb{Q}, a^2 < 2\}$, $B = \{b| b \in \mathbb{Q}, b^2 > 2\}$ and
    $c = 2$. Then $\sup A = \inf B = \sqrt{2}$ .

## section 1.4 The Consequence of the Axiom of Completeness

* **_1.4.1 Nested Interval Property_:** $I_n = [a_n, b_n]$ and $I_n \supseteq I_{n+1}$, then

$$
\displaystyle\cap_{i=1}^\infty I_i \neq \emptyset.
$$

* **_proof_:** Let $A = \{a_n\},B=\{b_n\}$. Let $x = \sup A$. Since every $b_n$ is an upper
bound of $A$, we have $x \le b_n$. Then $a_n \le x \le b_n$.
For every $n$, $x \in I_n$.

* **_1.4.2 Archimedean Property_:** 
(i) $x \in R$, then there exists $n \in N, n > x$.
(ii) $y > 0$, then there exists $n \in N, 1/n < y$.

* **_proof_:**
(i) Assume $N$ is bounded above, and $\alpha = \sup N$. Then there exists $n > \alpha -1$.
Then $n + 1 > \alpha$. We got a contradiction.
(ii) Let $x = 1/y$, and we find $n > x$, then $1/n < 1/x = y$.

* **_1.4.3 Density of Q in R_:** $a < b$, then exist rational number $r$, s.t. $a < r < b$.

(i) from 1.4.2, let $1/n < b-a$. Choose $m > an >= m-1$, then $a < m/n = (m-1)/n + 1/n \le a+1/n < b$.

* **_1.4.5 squre root in R_:** there exists $\alpha \in R$, such that $\alpha^2=2$.

* **_Exercise 1.4.1_** 

(a) Let $a = \frac{p}{q}, b=\frac{r}{s}$, then $a+b= \frac{ps+qr}{qs} \in \mathbb{Q}$.
(b) Let $b = a+t$, then $t = b + (-a)$. If $b \in \mathbb{Q}$, then $t \in \mathbb{Q}$,
    we have contradiction.
(c) Let $s = 2 + \sqrt{2}, t = 2-\sqrt{2},s+t=4,st=2$. $\mathbb{I}$ is not closed
    under addition and multiplication.

* **_Exercise 1.4.2_**

(a) First to prove $s$ is an upper bound of $A$. Let $a \in A$, if $a > s$, let $\epsilon = a - s > 0$.
Based on Archimedean Property, we can fine $n, s.t. 1/n < \epsilon$, then $s + 1/n < s + \epsilon=a$.
We have a contradiction.
(b) Second, if $s' < s$ is an upper bound, then $\epsilon = s - s'>0$, again we can find
$n, s.t. 1/n < \epsilon$, so $s'+1/n<s'+\epsilon=s$, so $s'<s-1/n$. Since $s-1/n$ is not an upper
bound of $A$, $s'$ cannot be as well. We have a contradiction.

* **_Exercise 1.4.3_**

(a) Assume $x \in \cap_{n=1}^{\infty}(0, 1/n)$. First $x \in (0,1)$, so $x > 0$.
Then according to Archimedean Property, we have $n, x > 1/n$, so $x \notin (0, 1/n)$.
We have a contradiction.

* **_Exercise 1.4.4_**

(a) Let $x \in [a,b] \cap \mathbb{Q}$, then $x \in [a,b]$, then $x \le b$, b is an upper bound.
(b) Let $a < c < b$, then according to 1.4.3, there exists $r \in Q$, s.t. $c < r < b$.
    Then $a < c < r < b$, so $r \in [a,b] \cap \mathbb{Q}$. $c$ is not an upper bound of $T$.
    Then $b = \sup T$.
    
* **_Exercise 1.4.5_** Given any real number $a < b$, there exists an irrational number $r$, such
that $a < r < b$.

(a) If a is irrational, we can find a rational number $a'$ such that $a < a' < b$. Same argument holds
for $b$. So we can assume $a, b$ are all rational.
(b) Now we can find $n$, s.t. $1/n < (b-a)/2$. Then we have $an < an + \sqrt{2} < an+2 < bn$.
Then we have $a < a + \sqrt{2}/n < b$. Since $a, 1/n$ are all rational, then $a + \sqrt{2}/n$
is irrational.
(c) A better proof: $a-\sqrt{2} < r < b-\sqrt{2}$.

* **_Exercise 1.4.6_**

(a) not dense
(b) dense
(c) Not dense. We can't find $p,q$ such $0 < p/q < 1/10$, which means $10|p| < q$

* **_Exercise 1.4.7_**

(a) $T = \{t \in R:  t^2 < 2\}$, $\alpha = \sup T$. Assume $\alpha ^ 2 > 2$, then
    $(\alpha - 1/n)^2 = \alpha^2 - 2\alpha/n + 1/n^2 > \alpha^2 - 2\alpha/n > 2$,
    if $n$ is big enough.
(b) On the other hand, we can find $t \in T$, such that $t > \alpha - 1/n$, so
    $t^2 > (\alpha - 1/n)^2 > 2$. We have a contradiction.

* **_Exercise 1.4.8_**

(a) Example: $A = \{r, r < 2, r \text{ is rational}\}$, $B = \{r, r < 2, r \text{ is irrational}\}$.
(b) Example: $J_i = \{ x : (-1/i, 1/i) \}$. We see $0 \in J_i$ and ${0} = \cap_{n=1}^{\infty} J_i$.
(c) Example: $L_i = [i, \infty)$
(d) Impossible: let $L_i = \cap_1^i J_i$, they are closed non-empty set, and they are nested.
    So based on "Nested Interval Property", $\cap_{n=1}^{\infty} J_i = \cap_{n=1}^{\infty} L_i$.

# Chapter 2 Sequences and Series

The crucial question is whether or not properties of addition and equality that are well understood for finite sums remain valid when applied to infinite objects such as equation.

## 2.2 The Limit of a Sequence

**_Definition 2.2.1_**. A sequence is a function whose domain is N.

**_Definition 2.2.3 Convergence of a Sequence)_**. A sequence $(a_n)$ converges to a real number $a$ if, for every positive number $ε$, there exists an $N ∈ \mathbb{N}$ such that whenever $n ≥ N$ it follows that $|a_n − a| < ε$.

**_Definition 2.2.4._** Given a real number $a ∈ R$ and a positive number $ε > 0$, the set
$$
V_{ε}(a)=\{x \in \mathbb{R} : |x-a| < ε\}
$$
is called the ε-neighborhood of $a$.

***Definition 2.2.3B (Convergence of a Sequence: Topological Version).*** A sequence $(a_n)$ converges to a if, given any ε-neighborhood $V_ε(a)$ of $a$, there exists a point in the sequence after which all of the terms are in $V_ε(a)$. In other words, every ε-neighborhood contains all but a finite number of the terms of $(a_n)$.

### Quantifiers

## 2.4 The Monotone Convergence Theorem and a First Look at Infinite Series

***Definition 2.4.1.*** A sequence $(a_{n})$ is *increasing* if $a_{n} \le a_{n+1}$
for all $n\in \mathbb{N}$ and *decreasing* if $a_{n} \ge a_{n+1}$ for all $n\in \mathbb{N}$. A sequence is *monotone* if it is either increasing or decreasing.

***Theorem 2.4.2 (Monotone Convergence Theorem).*** *If a sequence is monotone and bounded, then it converges.*

*Proof*: Let $s = \sup \{ a_{n} : n \in \mathbb{N} \}$.

***Definition 2.4.3 (Convergence of a Series).*** Let $(b_{n})$ be a sequence. An *infinite sequence* is a formal expression of the form

$$
\sum_{n=1}^{\infty} b_n = b_1 + b_2 + \cdots
$$

We define the corresponding *sequence of partial sums* ($s_m$) by

$$
s_m = b_1 + b_2 + \cdots + b_m,
$$

and say that the series $\sum_{n=1}^{\infty} b_n$ converges to $B$, if the sequence ($s_m$) converges to $B$. In this case, we write $\sum_{n=1}^{\infty} b_n = B$.

***Example 2.4.4.*** Consider
$$
\sum_{n=1}^{\infty} \frac{1}{n^2}
$$
We have
$$
s_m < (2 - \frac{1}{m}) < 2
$$
So we know it will converge.

***Example 2.4.5.*** Consider the so-called *harmonic series*
$$
\sum_{n=1}^{\infty} \frac{1}{n}
$$
We have
$$
s_{2^k} > 1 + k\left(\frac{1}{2}\right)
$$
***Theorem 2.4.6 (Cauchy Condensation Test).*** Suppose $(b_n)$ is decreasing and satisfies $(b_n) \ge 0$ for all $n\in \mathbb{N}$. Then, the series $\sum_{n=1}^{\infty} (b_n)$ converges if and only if the following series converges.

$$
\sum_{n=0}^{\infty} 2^n b_{2^n}
=
b_1 + 2 b_2 + 4 b_4 + \cdots
$$
***Corollary 2.4.7.*** The series $\sum_{n=1}^{\infty} 1 / n^p$ converges if and only if $p > 1$.

### Exercises

***Exercise 2.4.1.***

(a) Prove that the sequence defined by $x_1 = 3$ and

$$
x_{n+1} = \frac{1}{4-x_n}
$$

converges.

Proof: $x1 = 3, x_2 = 1, x_3 = 1/3, x_4 = 3/11$, assume $x_n < x_{n-1}$, then

$$
x_{n+1} = \frac{1}{4-x_n} < \frac{1}{4-x_{n-1}} < x_n
$$

And $x_n > 0$, so $(x_n)$ is monotonous decreasing and bounded. So it converges.

(b) Now that we know $\lim x_n$ exists, explain why $\lim x_{n+1}$ must also exist and equal the same value.

Proof: $x_{n+1}$ is also monotonous decreasing and bounded.

(c)

$$
x(4-x) = 1 \\
x^2 - 4x+1=0 \\
x = \frac{4 \pm \sqrt{12}}{2}
$$

***Exercise 2.4.2.***

(a) Consider the recursively defined sequence $y_1 = 1$,

$$
y_{n+1} = 3 - y_n
$$

and set $y = \lim y_n$. Because $(y_n)$ and $(y_{n+1})$ have the same limit, taking the limit across the recursive equation gives $y = 3-y$. Solving for
$y$, we conclude $y = \lim y_n = 3/2$. What is wrong with this argument?

Solution:

$$
y_n = 
\begin{cases}
1 & \quad \text{if } n \text{ is even} \\
2 & \quad \text{if } n \text{ is odd}
\end{cases}
$$
So $\lim y_n$ does not exist.

(b) This time set $y_1 = 1$ and $y_{n+1} = 3− \frac{1}{y_n}$. Can the strategy in (a) be applied $y_n$ to compute the limit of this sequence?

Solution: yes. $3 > y_2 > y_1 \ge 1$, and assume $3 > y_{n} > y_{n-1} \ge 1$, then 

$$
3 > 3 - \frac{1}{y_n} > 3 - \frac{1}{y_{n-1}} = y_n \ge 1
$$

So

$$
3 > y_{n+1} > y_n \ge 1
$$

so $(y_n)$ is monotonous increasing and bounded.

***Exercise 2.4.3.***

(a) Show that 

$$
\sqrt{2}, \sqrt{2+\sqrt{2}}, \sqrt{2+\sqrt{2+\sqrt{2}}}, \dots
$$
converges and find the limit.

Proof: let $b_1 = \sqrt{2}, b_2 = \sqrt{2+\sqrt{2}}$, then in general,
we have $b_{n+1} = \sqrt{2 + b_n}$. Because $b_2 > b_1$, and assume $b_n > b_{n-1}$, then $b_{n+1} = \sqrt{2 + b_n} > \sqrt{2+b_{n-1}} = b_n$.
So we prove this sequence is monotonous increasing.

Next, because $b_1 < 2$, and assume $b_n < 2$. Then we have $b_{n+1} = \sqrt{2+ b_n} < \sqrt{2+2} = 2$, so $b_n < 2, \forall n$. So this sequence is bounded.
So it converges.

Finally,

$$
b_{n+1}-2 = \sqrt{2+b_n}-2 =
\frac{2+b_n-4}{\sqrt{2+b_n}+2} =\\
\frac{b_n-2}{\sqrt{2+b_n}+2} < \\
\frac{b_n-2}{2} < \frac{b_1 - 2}{2^{n-1}}
$$
So we have $\lim b_n = 2$

(b) Does the sequence

$$
\sqrt{2}, \sqrt{2\sqrt{2}}, \sqrt{2\sqrt{2\sqrt{2}}}, \dots
$$
converge? If so, find the limit.

Proof: 

First, we show it's monotonous increasing. let $b1 = \sqrt{2}, b_2 = \sqrt{2\sqrt{2}}, b_3 = \sqrt{2\sqrt{2\sqrt{2}}}$, then in general, we have
$b_{n+1} = \sqrt{2b_n}$, because $b_2 > b_1$, and assume $b_n > b_{n-1}$, then
$b_{n+1} = \sqrt{2b_n} > \sqrt{2b_{n-1}} = b_n$.

Next we show it's upper bounded by 2. $b_1 < 2$ and assume $b_n < 2$, then
$b_{n+1} = \sqrt{2b_n} < \sqrt{2\times2} = 2$.

Finally, we show

$$
2 - b_{n+1} = 2 - \sqrt{2b_n} =\\
\frac{4-2b_n}{2+\sqrt{2b_n}} = \\
\frac{2-b_n}{1+\sqrt{\frac{b_n}{2}}} < \\
\frac{2-b_n}{1+\sqrt{\frac{b_1}{2}}} < \\
\frac{2-b_n}{1+\sqrt{\frac{1}{2}}} < \\
\frac{2-b_1}{(1+\sqrt{\frac{1}{2}})^{n-1}} \rightarrow 0
$$

***Exercise 2.4.4.*** 

(a) In Section 1.4 we used the Axiom of Completeness (AoC) to prove the Archimedean Property of $\mathbb{R}$ (Theorem 1.4.2). Show that the Monotone Convergence Theorem can also be used to prove the Archimedean Property without making any use of AoC.

**_1.4.2 Archimedean Property_:** 
(i) $x \in R$, then there exists $n \in N, n > x$.
(ii) $y > 0$, then there exists $n \in N, 1/n < y$.

Proof: Assume $\mathbb{N}$ is bounded, then we can assume $\lim n = a$.
Now $a-1$ is not a upper bound for $\mathbb{N}$, we can find $n$, such that
$n > a-1$, than means $n+1 > a$. We have an contradiction.

(b) Use the Monotone Convergence Theorem to supply a proof for the Nested Interval Property (Theorem 1.4.1) that doesn’t make use of AoC.

* **_1.4.1 Nested Interval Property_:** $I_n = [a_n, b_n]$ and $I_n \supseteq I_{n+1}$, then

$$
\displaystyle\cap_{i=1}^\infty I_i \neq \emptyset.
$$

Proof: $\{a_n\}$ is monotonous increasing and bounded, so we can assume $\lim a_n = a$. If $b_m < a$, then we can find $n$, such that $n > m$ and $b_m < a_n < b_n < a$. However, $\{b_n\}$ is monotonous decreasing, so we must have $b_n <= b_m$, then we have a contradiction. Therefore, $b_m >= a, \forall m$.
So $a \in I_i, \forall i$.

***Exercise 2.4.5 (Calculating Square Roots).*** Let $x_1 = 2$, and define

$$
x_{n+1} = \frac{1}{2}(x_n + \frac{2}{x_n})
$$

(a) Show that $x^2$ is always greater than or equal to 2, and then use this to
prove that $x_{n} − x_{n+1} ≥ 0$. Conclude that $\lim x_n = \sqrt{2}$.

Proof: 

$$
x_{n+1}^2 - 2 = \frac{1}{2}(x_n + \frac{2}{x_n})^2 - 2
= \frac{1}{4}(x_n^2 + 4 + \frac{4}{x_n^2}) - 2
\ge \frac{1}{x_n^2} 
\ge 0
$$
$$
x_{n} − x_{n+1} = \frac{1}{2}(x_n - \frac{2}{x_n}) \ge 0
$$

$$
x_{n+1} - \sqrt{2} = \frac{1}{2}(x_n-2\sqrt{2}+\frac{2}{x_n})
= \frac{1}{2} (\sqrt{x_n} - \frac{\sqrt{2}}{\sqrt{x_n}})^2\\
= \frac{1}{2} \frac{(x_n - \sqrt{2})^2}{x_n} \\
= \frac{1}{2} (x_n - \sqrt{2}) \frac{x_n - \sqrt{2}}{x_n} \\
\le \frac{1}{2} (x_n - \sqrt{2}) \le \frac{1}{2^{n-1}} (2 - \sqrt{2})
$$

So $\lim x_n = \sqrt{2}$.

***Exercise 2.4.6. (Arithmetic–Geometric Mean). *** (a) Explain why $\sqrt{xy} \le (x+y)/2$ for any two positive real numbers x and y.

Proof:

$$
x + y - 2\sqrt{xy} = (\sqrt{x} - \sqrt{y})^2 \ge 0
$$
So $\sqrt{xy} \le (x+y)/2$.

(b) Now let $0≤ x_1 ≤ y_1$ and define

$$
x_{n+1} = \sqrt{x_ny_n} \quad \text{and} \quad y_{n+1} = \frac{x_n+y_n}{2}
$$

Show $lim x_n$ and $lim y_n$ both exist and are equal.

Proof: $x_{n+1} = \sqrt{x_ny_n} \ge \sqrt{x_nx_n} = x_n$ and 
$y_{n+1} \le \frac{y_n+y_n}{2} = y_n$, so $x_n$ is monotonous increasing,
and $y_n$ is monotonous decreasing. And they are bounded.
So $lim x_n$ and $lim y_n$ both exist.

$$
y_{n+1} - x_{n+1} = \frac{1}{2}(\sqrt{y_n} - \sqrt{x_n})^2 \le
\frac{1}{2}(\sqrt{y_n} - \sqrt{x_n})(\sqrt{y_n} + \sqrt{x_n}) =
\frac{y_n - x_n}{2} \le \frac{y_1 - x_1}{2^{n-1}}
$$

So $\lim y_n - \lim x_n = 0$.

***Exercise 2.4.7. (Limit Superior). *** Let $(a_{n})$ be a bounded sequence.

(a) Prove that the sequence defined by $y_n = \sup \{a_k : k ≥ n\}$ converges.

Proof: $y_n$ is a monotonous decreasing. And $y_n \ge \inf \{(a_n)\}$, so
$y_n$ is bounded. So $y_n$ converges.

(b) The limit superior of $(a_{n})$, or $\lim \sup a_n$ , is defined by

$$
\lim \sup a_n = \lim y_n
$$

where $y_n$ is the sequence from part (a) of this exercise. Provide a reason- able definition for $\lim \inf a_n$ and briefly explain why it always exists for any bounded sequence.

Solution: let $x_n = \inf \{a_k : k ≥ n\}$, then define:

$$
\lim \inf a_n = \lim x_n
$$

(c) Prove that $\lim \inf a_n ≤ \lim \sup a_n$ for every bounded sequence, and give an example of a sequence for which the inequality is strict.

Proof: Because $x_n \le y_n$, according to Theorem 2.3.4 (Order Limit Theorem),
we have $\lim \inf a_n ≤ \lim \sup a_n$. Consider the following sequence

$$
a_n = 
\begin{cases}
0 & \quad \text{if } n \text{ is even} \\
1 & \quad \text{if } n \text{ is odd}
\end{cases}
$$

(d) Show that $\lim \inf a_n = \lim \sup a_n$ if and only if $\lim a_n$ exists. In this case, all three share the same value.

Proof: **only if**: let $\lim \inf a_n = \lim \sup a_n = a$, for any $\epsilon$, we can find
a $N$, such that $a - \epsilon < y_n < a < x_n < a + \epsilon, \forall n > N$, and this means
$a - \epsilon < a_n < a + \epsilon, \forall n > N$, i.e. $|a_n - a| < \epsilon$ for all $n > N$.

Another kind of problematic method, because $y_n \le a_n \le x_n$, so
$\lim y_n \le \lim a_n \le \lim x_n$.

**if**: On the other hand, assume $\lim a_n = a$, then for any $\epsilon$, we can find
$N$ s.t. as long as $n > N$, $a_n < a + \epsilon$, that means $x_n \leq a + \epsilon$ for all $n > N$. So it's not possible that $\lim x_n > a$. So we have $\lim x_n \le a$. For the same reason,
$\lim y_n \ge a$. Using (c), we have  $\lim x_n \ge \lim y_n$. So we have
$\lim \inf a_n = \lim \sup a_n = a$.

***Exercise 2.4.8. *** For or each series, find an explicit formula for the sequence of partial sums and determine if the series converges.

(a)

$$
\sum_{n=1}^{\infty} \frac{1}{2^n}
$$
$$
\sum_{n=1}^{m} \frac{1}{2^n} = 1 - \frac{1}{2^m} \rightarrow 1
$$
(b)

$$
\sum_{n=1}^{\infty} \frac{1}{n(n+1)}
$$
$$
\sum_{n=1}^{m} \frac{1}{n(n+1)} = 1 - \frac{1}{m+1} \rightarrow 1
$$
(c)

$$
\sum_{n=1}^{\infty} \log (\frac{n+1}{n})
$$
$$
\sum_{n=1}^{m} \log (\frac{n+1}{n}) = \log (m+1) \rightarrow \infty
$$

***Exercise 2.4.9. *** Complete the proof of Theorem 2.4.6 by showing that if the series $\sum_{n=0}^{\infty} 2^n b_{2^n}$ diverges, then so does $\sum_{n=1}^{\infty} (b_n)$.

Proof: We have $2b_1 > s_1-b1, 2(b1 + b2 + b3) > s_2-b1, 2(b1+\cdots+b_7) > s_3-b1$. If $\sum_{n=0}^{\infty} 2^n b_{2^n}$, $\sum_{n=1}^{\infty} (b_n)$ is also unbounded.

***Exercise 2.4.10 (Infinite Products). *** A close relative of infinite series is the infinite product

$$
\prod_{n=1}^{\infty}
b_n = b_1 b_2\cdots
$$
which is understood in terms of its sequence of partial products

$$
p_m =
\prod_{n=1}^{m} b_n
=
b_1 b_2 \cdots b_m
$$
Consider the special class of infinite products of the form

$$
\prod_{n=1}^{\infty} (1 + a_n) \quad \text{where } a_n \ge 0.
$$
(a) Find an explicit formula for the sequence of partial products in the case where $a_n = 1/n$ and decide whether the sequence converges. Write out the first few terms in the sequence of partial products in the case where $a_n = 1/n^2$ and make a conjecture about the convergence of this sequence.

Solution: 

$$
p_m = 
(1 + 1) * (1 + \frac{1}{2}) * \cdots * (1 + \frac{1}{m})
= 2 \cdot \frac{3}{2} \cdots \frac{m+1}{m} = m+1
$$
So it's not converging.

$$
p_m = (1 + 1) * (1 + \frac{1}{4}) * \cdots * (1 + \frac{1}{m^2}) \\
= 2 * \frac{5}{4} * \frac{10}{9} * \cdots * \frac{m^2+1}{m^2} \\
$$

So $p_1 = 2, p_2 = 2.5, p_3 = 2.78, P_4 = 2.95$


(b) Show, in general, that the sequence of partial products converges if and only if $\sum_{n=1}^{\infty} (a_n)$ converges. (The inequality $1 + x ≤ 3^x$ for positive x will be useful in one direction.)

Proof: Assume $\sum_{n=1}^{\infty} (a_n)$ converges, then $p_m = \prod_{n=1}^{m} (1 + a_m) < 3^{a_1a_2 \dots a_m} < 3^M$, so $p_m$ is bounded.

On the other hand assume $\prod_{n=1}^{\infty} (1 + a_n)$ converges, then
$p_m > a_1 + a_2 + \cdots + a_m$, which can be proved by induction. Then
$a_1 + a_2 + \cdots + a_m$ is bounded and it converges.

# Chapter -1 Commonly used symbols

$$
\mathbb{R}, \\
ε \\
\cap_{n=1}^{\infty} \\
(a_{n}) , (b_{n}) n\in \mathbb{N} \\
\sum_{n=1}^{\infty} \\
\prod_{n=1}^{\infty} \\
\frac{1}{n}, \frac{1}{n^2} \\
\forall n > N 
$$

## Solution manuals

* [linearalgebras.com](https://linearalgebras.com/solution-understanding-analysis.html)
* [github](https://github.com/mikinty/Understanding-Analysis-Abbott-Solutions)


